examples/Cancel/Monoid.v
@@ -7,20 +7,20 @@ Parameter N : nat -> M.
 Local Infix "&" := P (at level 50).
 Local Infix "%is" := R (at level 70).
 
-Axiom plus_unit_p : forall a b, a %is b -> U & a %is b.
-Axiom plus_assoc_p1 : forall a b c d,
+Axiom plus_unit_p : forall b a, a %is b -> U & a %is b.
+Axiom plus_assoc_p1 : forall d c b a,
     a & (b & c) %is d -> (a & b) & c %is d.
-Axiom plus_assoc_p2 : forall a b c d,
+Axiom plus_assoc_p2 : forall d c b a,
     b & (a & c) %is d -> (a & b) & c %is d.
-Axiom plus_comm_p : forall a b c, a & b %is c -> b & a %is c.
+Axiom plus_comm_p : forall c b a, a & b %is c -> b & a %is c.
 
-Axiom plus_unit_c : forall a b, a %is b -> a %is U & b.
-Axiom plus_assoc_c1 : forall a b c d,
+Axiom plus_unit_c : forall b a, a %is b -> a %is U & b.
+Axiom plus_assoc_c1 : forall d c b a,
     d %is a & (b & c) -> d %is (a & b) & c.
-Axiom plus_assoc_c2 : forall a b c d,
+Axiom plus_assoc_c2 : forall d c b a,
     d %is b & (a & c) -> d %is (a & b) & c.
-Axiom plus_comm_c : forall a b c, c %is a & b -> c %is b & a.
-Axiom plus_cancel : forall a b c d, a %is c -> b %is d -> a & b %is c & d.
+Axiom plus_comm_c : forall c b a, c %is a & b -> c %is b & a.
+Axiom plus_cancel : forall d c b a, a %is c -> b %is d -> a & b %is c & d.
 
 Axiom refl : forall a, a %is a.
 
