theories/Lemma.v
@@ -29,8 +29,7 @@ Section lem.
   Fixpoint foralls (ls : list typ) : (OpenT typD ls Prop) -> Prop :=
     match ls as ls return (OpenT typD ls Prop) -> Prop with
       | nil => fun P => P Hnil
-      | l :: ls => fun P => forall x : typD l,
-                              foralls (fun z => P (Hcons x z))
+      | l :: ls => fun P => foralls (fun z => forall x : typD l, P (Hcons x z))
     end.
 
   Lemma foralls_sem : forall ls P,
@@ -41,9 +40,8 @@ Section lem.
     { intuition; rewrite hlist_eta; auto. }
     { intuition.
       { rewrite hlist_eta.
-        specialize (H (hlist_hd h)).
-        rewrite IHls in H. eauto. }
-      { rewrite IHls. intuition. } }
+        eapply IHls in H. eapply H. }
+      { eapply IHls. eauto. } }
   Qed.
 
   Lemma foralls_iff
@@ -109,6 +107,49 @@ Section lem.
       | _ , _ => None
     end.
 
+(*   Fixpoint rev_app_distr_trans {T} (a b : list T) : rev (a ++ b) = rev b ++ rev a. *)
+(*   destruct a. *)
+(*   { simpl. rewrite app_nil_r_trans. reflexivity. } *)
+(*   { simpl. rewrite rev_app_distr_trans. *)
+(*     rewrite app_ass_trans. reflexivity. } *)
+(*   Defined. *)
+(* About app_nil_r_trans. *)
+
+(*   Fixpoint rev_involutive_trans {T} (a : list T) : rev (rev a) = a. *)
+(*   refine *)
+(*     match a as a return rev (rev a) = a with *)
+(*     | nil => _ *)
+(*     | x :: xs => _ *)
+(*     end. *)
+(*   { reflexivity. } *)
+(*   { simpl. rewrite rev_app_distr_trans. rewrite rev_involutive_trans. *)
+(*     reflexivity. } *)
+(*   Defined. *)
+
+(*   Definition lemmaD'' (tus tvs : tenv typ) (l : lemma) *)
+(*   : option (exprT tus tvs Prop) := *)
+(*     match *)
+(*         Traversable.mapT (T := list) (F := option) *)
+(*                          (fun e : expr => exprD'_typ0 tus (vars l ++ tvs) e) *)
+(*                          (premises l) *)
+(*       , conclusionD tus (vars l ++ tvs) (concl l) *)
+(*     with *)
+(*       | Some prems , Some concl => *)
+(*         Some (fun us vs => *)
+(*                 foralls (fun h : hlist (typD) (rev (vars l)) => *)
+(*                            let h : hlist typD (vars l) := *)
+(*                                match rev_involutive_trans (vars l) *)
+(*                                      in _ = X return hlist _ X *)
+(*                                with *)
+(*                                | eq_refl => hlist_rev h *)
+(*                                end in *)
+(*                            let vs' := hlist_app h vs in *)
+(*                            impls (map (fun x => x us vs') prems) *)
+(*                                  (concl us vs'))) *)
+(*       | _ , _ => None *)
+(*     end. *)
+
+
   Hypothesis conclusionD_weaken
   : forall tus tvs l lD,
       conclusionD tus tvs l = Some lD ->
@@ -117,7 +158,6 @@ Section lem.
           conclusionD (tus ++ tus') (tvs ++ tvs') l = Some lD' /\
           forall us us' vs vs',
             lD us vs <-> lD' (hlist_app us us') (hlist_app vs vs').
-
 
   Opaque Traversable.mapT.
 
